proofs/xor_key1_state.lean
@@ -1,0 +1,67 @@
+
+-- Experimental lean backend for Hax
+-- The Hax prelude library can be found in hax/proof-libs/lean
+import Hax
+import Std.Tactic.Do
+import Std.Do.Triple
+import Std.Tactic.Do.Syntax
+import Utilities
+open Std.Do
+open Std.Tactic
+
+set_option mvcgen.warning false
+set_option linter.unusedVariables false
+
+
+namespace aes_core.xor_key1_state
+
+def xor_key1_state_spec (st : (Vector u16 8)) (k : (Vector u16 8)) : (Vector u16 8) :=
+  (Vector.zip st k).map (fun (x, y) => x ^^^ y)
+
+@[spec]
+def xor_key1_state (st : (RustArray u16 8)) (k : (RustArray u16 8)) :
+    RustM (RustArray u16 8) := do
+  let st : (RustArray u16 8) ←
+    (rust_primitives.hax.monomorphized_update_at.update_at_usize
+      st
+      (0 : usize)
+      (← ((← st[(0 : usize)]_?) ^^^? (← k[(0 : usize)]_?))));
+  let st : (RustArray u16 8) ←
+    (rust_primitives.hax.monomorphized_update_at.update_at_usize
+      st
+      (1 : usize)
+      (← ((← st[(1 : usize)]_?) ^^^? (← k[(1 : usize)]_?))));
+  let st : (RustArray u16 8) ←
+    (rust_primitives.hax.monomorphized_update_at.update_at_usize
+      st
+      (2 : usize)
+      (← ((← st[(2 : usize)]_?) ^^^? (← k[(2 : usize)]_?))));
+  let st : (RustArray u16 8) ←
+    (rust_primitives.hax.monomorphized_update_at.update_at_usize
+      st
+      (3 : usize)
+      (← ((← st[(3 : usize)]_?) ^^^? (← k[(3 : usize)]_?))));
+  let st : (RustArray u16 8) ←
+    (rust_primitives.hax.monomorphized_update_at.update_at_usize
+      st
+      (4 : usize)
+      (← ((← st[(4 : usize)]_?) ^^^? (← k[(4 : usize)]_?))));
+  let st : (RustArray u16 8) ←
+    (rust_primitives.hax.monomorphized_update_at.update_at_usize
+      st
+      (5 : usize)
+      (← ((← st[(5 : usize)]_?) ^^^? (← k[(5 : usize)]_?))));
+  let st : (RustArray u16 8) ←
+    (rust_primitives.hax.monomorphized_update_at.update_at_usize
+      st
+      (6 : usize)
+      (← ((← st[(6 : usize)]_?) ^^^? (← k[(6 : usize)]_?))));
+  let st : (RustArray u16 8) ←
+    (rust_primitives.hax.monomorphized_update_at.update_at_usize
+      st
+      (7 : usize)
+      (← ((← st[(7 : usize)]_?) ^^^? (← k[(7 : usize)]_?))));
+  (pure st)
+
+
+end aes_core.xor_key1_state
